Remove name gen
Changes from September that were not committed.

PyLevelLang/src/PyLevelLang/Compile.v
@@ -7,7 +7,6 @@ Require Import coqutil.Datatypes.Result.
 Import ResultMonadNotations.
 Require Import coqutil.Map.Interface coqutil.Map.SortedListString coqutil.Map.MapEauto.
 Require Import coqutil.Byte coqutil.Word.Interface coqutil.Word.Bitwidth coqutil.Word.Properties.
-Require Import compiler.NameGen.
 
 Require Import coqutil.Tactics.Tactics.
 Require Import coqutil.Tactics.fwd.
@@ -32,7 +31,7 @@ Definition compile_unop {t1 t2 : type} (o : unop t1 t2) :
   | OFst _ _ _
   | OSnd _ _ _
   | OIntToString =>
-      error:("unimplemented")
+      error:("unsupported")
   end.
 
 Definition compile_binop {t1 t2 t3 : type} (o : binop t1 t2 t3) :
@@ -54,7 +53,7 @@ Definition compile_binop {t1 t2 t3 : type} (o : binop t1 t2 t3) :
       Success (Syntax.expr.op Syntax.bopname.or)
   | OConcat _
   | OConcatString =>
-      error:("unimplemented")
+      error:("unsupported")
   | OWLessU =>
       Success (Syntax.expr.op Syntax.bopname.ltu)
   | OWLessS =>
@@ -74,46 +73,26 @@ Definition compile_binop {t1 t2 t3 : type} (o : binop t1 t2 t3) :
   | OCons _
   | ORange
   | OWRange =>
-      error:("unimplemented")
+      error:("unsupported")
   end.
 
-Section NameGen.
-  Context {NGstate : Type}
-          {NG : NameGen string NGstate}
-          {namemap : map.map string string}
-          {namemap_ok : map.ok namemap}.
-
-  Fixpoint compile_expr {t : type} (e : expr t) (nm : namemap) (st : NGstate) :
-    result (Syntax.cmd * Syntax.expr * namemap * NGstate) :=
-    match e with
-    | EVar _ x | ELoc _ x =>
-        match map.get nm x with
-        | Some x' =>
-            Success (Syntax.cmd.skip, Syntax.expr.var x', nm, st)
-        | None =>
-            error:("variable" x "not mapped in target language (unreachable)")
-        end
-    | EAtom a =>
-        e' <- compile_atom a;;
-        Success (Syntax.cmd.skip, e', nm, st)
-    | EUnop o e1 =>
-        f <- compile_unop o;;
-        '(c1, e1', _, _) <- compile_expr e1 nm st;;
-        Success (c1, f e1', nm, st)
-    | EBinop o e1 e2 =>
-        f <- compile_binop o;;
-        '(c1, e1', _, _) <- compile_expr e1 nm st;;
-        '(c2, e2', _, _) <- compile_expr e2 nm st;;
-        Success (Syntax.cmd.seq c1 c2, f e1' e2', nm, st)
-    | ELet x e1 e2 =>
-        '(c1, e1', _, _) <- compile_expr e1 nm st;;
-        '(c2, e2', _, _) <- compile_expr e2 nm st;;
-        let '(x', st') := genFresh st in
-        let nm' := map.put nm x x' in
-        Success (Syntax.cmd.seq c1 (Syntax.cmd.seq (Syntax.cmd.set x' e1') c2), e2', nm', st')
-    | _ => error:("unimplemented")
-    end.
-End NameGen.
+Fixpoint compile_expr {t : type} (e : expr t) : result Syntax.expr :=
+  match e with
+  | EVar _ x | ELoc _ x =>
+      Success (Syntax.expr.var x)
+  | EAtom a =>
+      compile_atom a
+  | EUnop o e1 =>
+      f <- compile_unop o;;
+      e1' <- compile_expr e1;;
+      Success (f e1')
+  | EBinop o e1 e2 =>
+      f <- compile_binop o;;
+      e1' <- compile_expr e1;;
+      e2' <- compile_expr e2;;
+      Success (f e1' e2')
+  | _ => error:("unsupported")
+  end.
 
 Section WithMap.
   Context {width : Z} {BW : Bitwidth width} {word : word.word width} {mem : map.map word byte}
@@ -122,11 +101,7 @@ Section WithMap.
           {locals : map.map string {t & interp_type (word := word) t}} {locals_ok : map.ok locals}
           {locals' : map.map string word} {locals'_ok : map.ok locals'}
           {env : map.map String.string (list String.string * list String.string * Syntax.cmd)}
-          {ext_spec : ExtSpec}
-          {NGstate : Type}
-          {NG : NameGen string NGstate}
-          {namemap : map.map string string}
-          {namemap_ok : map.ok namemap}.
+          {ext_spec : ExtSpec}.
 
   (* Relation between source language and target language values,
    * denoting that two values are equivalent for a given type *)
@@ -144,69 +119,65 @@ Section WithMap.
   (* Relation between source language and target language locals maps,
    * denoting that the source language locals are a "subset" of the target
    * language locals *)
-  Definition locals_relation (lo : locals) (l : locals') (nm : namemap) : Prop :=
+  Definition locals_relation (lo : locals) (l : locals') : Prop :=
     map.forall_keys (fun x =>
-    match map.get lo x, map.get nm x with
-    | Some (existT _ _ val), Some x' =>
-        match map.get l x' with
+    match map.get lo x with
+    | Some (existT _ _ val) =>
+        match map.get l x with
         | Some val' => value_relation val val'
         | None => False
         end
-    | _, _ => True
+    | _ => True
     end) lo.
 
-  Lemma locals_relation_extends (lo : locals) (l l' : locals') (nm : namemap) :
-    map.extends l' l -> locals_relation lo l nm -> locals_relation lo l' nm.
+  Lemma locals_relation_extends (lo : locals) (l l' : locals') :
+    map.extends l' l -> locals_relation lo l -> locals_relation lo l'.
   Proof.
     intros Hex.
     apply weaken_forall_keys.
-    intros key Hl.
+    intros x Hl.
     destruct map.get as [s|]; try easy.
     destruct s as [t val].
-    destruct (map.get nm key) as [x'|]; try easy.
-    destruct (map.get l x') as [v|] eqn:E.
+    destruct (map.get l x) as [v|] eqn:E.
     - apply (Properties.map.extends_get (m1 := l) (m2 := l')) in E;
       [| assumption].
       now rewrite E.
     - destruct Hl.
   Qed.
 
-  Lemma locals_relation_get (lo : locals) (l : locals') (nm : namemap) :
-    locals_relation lo l nm ->
-    forall (x x' : string) (t : type) (s : {t & interp_type t}),
-    map.get lo x = Some s ->
-    map.get nm x = Some x' -> exists (w : word),
-    map.get l x' = Some w.
+  Lemma locals_relation_get (lo : locals) (l : locals') :
+    locals_relation lo l ->
+    forall (x : string) (t : type) (s : {t & interp_type t}),
+    map.get lo x = Some s -> exists (w : word),
+    map.get l x = Some w.
   Proof.
-    intros Hl x x' t s Hs Hx'.
+    intros Hl x t s Hs.
     unfold locals_relation, map.forall_keys in Hl.
     specialize Hl with (1 := Hs).
     rewrite Hs in Hl.
     destruct map.get.
     - fwd. now exists r.
-    - discriminate Hx'.
+    - destruct s, Hl.
   Qed.
 
-  Lemma locals_relation_put (lo : locals) (l : locals') (nm : namemap) :
-    locals_relation lo l nm ->
-    forall (x x' : string) (t : type) (v : interp_type t) (w : word),
+  Lemma locals_relation_put (lo : locals) (l : locals') :
+    locals_relation lo l ->
+    forall (x : string) (t : type) (v : interp_type t) (w : word),
     value_relation v w ->
-    map.get nm x = Some x' ->
-    locals_relation (set_local lo x v) (map.put l x' w) nm.
+    locals_relation (set_local lo x v) (map.put l x w).
   Proof.
-  Admitted.
-  (*   intros Hl x t v w Hvw. *)
-  (*   unfold locals_relation, map.forall_keys, set_local. *)
-  (*   intros x' [t' v']. *)
-  (*   repeat rewrite Properties.map.get_put_dec. *)
-  (*   destruct (x =? x')%string. *)
-  (*   - easy. *)
-  (*   - intros Hx'. fwd. *)
-  (*     unfold locals_relation, map.forall_keys in Hl. *)
-  (*     specialize Hl with (1 := Hx'). *)
-  (*     rewrite Hx' in Hl. *)
-  (*     assumption. *)
-  (* Qed. *)
+    intros Hl x t v w Hvw.
+    unfold locals_relation, map.forall_keys, set_local.
+    intros x' [t' v'].
+    repeat rewrite Properties.map.get_put_dec.
+    destruct (x =? x')%string.
+    - easy.
+    - intros Hx'. fwd.
+      unfold locals_relation, map.forall_keys in Hl.
+      specialize Hl with (1 := Hx').
+      rewrite Hx' in Hl.
+      assumption.
+  Qed.
 
   Definition tenv_relation (G : tenv) (lo : locals) : Prop :=
     map.forall_keys (fun key =>
@@ -317,81 +288,73 @@ Section WithMap.
         now rewrite H2.
   Qed.
 
+  Compute (compile_expr (EBinop (OEq _ _) (EAtom (ABool true)) (EAtom (ABool false)))).
+
   Lemma compile_correct :
-    forall {t} (e : expr t) (c : Syntax.cmd) (e' : Syntax.expr)
-    (G : tenv) (lo : locals) (nm nm' : namemap) (st st' : NGstate),
-    tenv_relation G lo ->
+    forall {t} (e : expr t) (e' : Syntax.expr) (G : tenv),
     wf G e ->
-    compile_expr e nm st = Success (c, e', nm', st') -> forall tr m l,
-    locals_relation lo l nm ->
-    locals_relation lo l nm' /\
-    exec map.empty c tr m l (fun tr' m' l' => exists (w : word),
-      eval_expr m' l' e' = Some w /\
-      value_relation (interp_expr lo e) w /\
-      m' = m /\
-      map.extends l' l
-    ).
+    compile_expr e = Success e' -> forall lo l,
+    tenv_relation G lo ->
+    locals_relation lo l -> exists w : word, forall m,
+    eval_expr m l e' = Some w /\
+    value_relation (interp_expr lo e) w.
   Proof.
-    intros t. induction e; intros c e' G lo nm nm' st st' Hlo He He' tr m l Hl; try easy.
+    intros t. induction e; intros e' G He He' lo l Hlo Hl; try easy.
     1-2:
       (* EVar x, ELoc x *)
       unfold compile_expr in He';
       fwd;
       simpl;
-      rename s into x';
-      split; [easy |];
-      apply exec.skip;
       inversion_clear He;
       destruct (tenv_relation_get _ lo Hlo _ _ _ H) as [v Hv];
-      destruct (locals_relation_get _ l _ Hl  _ x' t _ Hv) as [w Hw]; [easy |];
+      destruct (locals_relation_get _ l Hl x t _ Hv) as [w Hw];
       exists w;
-      ssplit; try easy;
+      intros m; ssplit; try easy;
       unfold get_local;
       rewrite Hv;
       unfold locals_relation, map.forall_keys in Hl;
       specialize Hl with (1 := Hv);
-      rewrite Hv, E, Hw in Hl;
+      rewrite Hv, Hw in Hl;
       now rewrite <- proj_expected_existT.
     - (* EAtom a *)
       unfold compile_expr in He'.
       fwd.
-      split; [easy |].
-      apply exec.skip.
+      simpl.
       destruct a; try easy.
       + (* AInt n *)
-        injection E as [= <-].
         simpl.
+        simpl in He'.
+        fwd.
         exists (word.of_Z (word.wrap n)).
-        ssplit; try easy;
+        intros m; ssplit;
         rewrite <- word.unsigned_of_Z, word.of_Z_unsigned; try easy.
         apply RWord.
       + (* ABool b *)
-        injection E as [= <-].
         simpl.
+        simpl in He'.
+        fwd.
         exists (word.of_Z (Z.b2z b)).
-        ssplit; try easy.
+        intros m; ssplit; try easy.
         apply RBool.
     - (* EUnop o e *)
       destruct o; try easy.
       all:
-        simpl in He';
         simpl;
-        fwd;
+        simpl in He';
+        fwd; rename a into e', E into He';
         inversion He;
-        apply Eqdep_dec.inj_pair2_eq_dec in H4 as [= ->]; try exact type_eq_dec;
-        specialize IHe with (1 := Hlo) (2 := H2) (3 := E);
-        split; [easy |];
-        eapply exec.weaken; [ now apply IHe |];
-        cbv beta;
-        intros tr' m' l' Hw;
+        apply Eqdep_dec.inj_pair2_eq_dec in H3, H4 as [= ->]; try exact type_eq_dec;
+        apply Eqdep_dec.inj_pair2_eq_dec in H3 as [= ->]; try exact type_eq_dec;
+        subst;
+        specialize IHe with (1 := H2) (2 := eq_refl) (3 := Hlo) (4 := Hl);
         fwd;
         eexists;
-        ssplit;
-        [ simpl; now fwd
-        |
-        | reflexivity
-        | assumption ];
-        inversion Hwp1;
+        intros m; specialize IHe with m; fwd;
+        simpl;
+        rewrite IHep0;
+        split;
+        [ reflexivity |];
+        inversion IHep1;
         subst;
         repeat (repeat lazymatch goal with
         | h: existT _ _ _ = existT _ _ _ |- _ =>
@@ -407,44 +370,33 @@ Section WithMap.
     - (* EBinop o e1 e2 *)
       destruct o; try easy.
       all:
-        simpl in He';
         simpl;
-        fwd;
+        simpl in He';
+        fwd; rename a into e1', E into He1', a0 into e2', E0 into He2';
         inversion He;
-        apply Eqdep_dec.inj_pair2_eq_dec in H5 as [= ->]; try exact type_eq_dec;
-        injection H6 as [= ->];
-        apply Eqdep_dec.inj_pair2_eq_dec in H5 as [= ->]; try exact type_eq_dec;
-        specialize IHe1 with (1 := Hlo) (2 := H3) (3 := E);
-        specialize IHe2 with (1 := Hlo) (2 := H7) (3 := E0);
-        split; [easy |];
-        eapply exec.seq; [ now apply IHe1 |];
-        cbv beta;
-        intros tr' m' l' Hw;
-        fwd;
-        eapply exec.weaken; [
-          apply IHe2;
-          assumption || now apply locals_relation_extends with (l := l)
-        |];
-        cbv beta;
-        intros tr'' m'' l'' Hw';
-        fwd;
-        eexists;
-        ssplit;
-        [ simpl; fwd;
-          apply eval_map_extends_locals with (l' := l'') in Hwp0;
-          [| assumption];
-          now rewrite Hwp0
-        |
-        | reflexivity
-        | now apply extends_trans with l' ].
-      1-9:
-        inversion Hwp1; inversion Hw'p1;
-        subst;
-        repeat lazymatch goal with
+        repeat (repeat lazymatch goal with
         | h: existT _ _ _ = existT _ _ _ |- _ =>
             apply interp_type_eq in h
         end;
+        subst);
+        apply Eqdep_dec.inj_pair2_eq_dec in H5, H6 as [= ->]; try exact type_eq_dec;
         subst;
+        specialize IHe1 with (1 := H3) (2 := eq_refl) (3 := Hlo) (4 := Hl);
+        specialize IHe2 with (1 := H7) (2 := eq_refl) (3 := Hlo) (4 := Hl);
+        fwd;
+        eexists;
+        intros m; specialize IHe1 with m; specialize IHe2 with m; fwd;
+        simpl;
+        rewrite IHe1p0, IHe2p0;
+        split;
+        [ reflexivity |];
+        inversion IHe1p1; inversion IHe2p1;
+        subst;
+        repeat (repeat lazymatch goal with
+        | h: existT _ _ _ = existT _ _ _ |- _ =>
+            apply interp_type_eq in h
+        end;
+        subst);
         set (v1 := interp_expr _ e1);
         set (v2 := interp_expr _ e2).
       1-5:
@@ -467,7 +419,37 @@ Section WithMap.
       + (* OWLessS *)
         destruct (word.lts v1 v2);
         apply RBool.
-      + (* OEq *)
+      + (* OEq TWord _ *)
+        unfold eqb_values.
+        inversion IHe1p1; inversion IHe2p1.
+        subst.
+        repeat (repeat lazymatch goal with
+        | h: existT _ _ _ = existT _ _ _ |- _ =>
+            apply interp_type_eq in h
+        end;
+        subst).
+        destruct (word.eqb _ _);
+        apply RBool.
+      + (* NOT OEq TBool _ *)
+        unfold eqb_values.
+        inversion IHe1p1; inversion IHe2p1.
+        subst.
+        repeat (repeat lazymatch goal with
+        | h: existT _ _ _ = existT _ _ _ |- _ =>
+            apply interp_type_eq in h
+        end;
+        subst).
+        rewrite <- H8.
+          set (b1 := interp_expr _ e1).
+          set (b2 := interp_expr _ e2).
+          destruct b1, b2.
+          (* all: *)
+          (*   apply RBool'; *)
+          (*   simpl; *)
+          (*   rewrite word.unsigned_eqb; *)
+          (*   try rewrite word.unsigned_of_Z_0; *)
+          (*   now try rewrite word.unsigned_of_Z_1. *)
+          
         destruct t;
         try easy; unfold eqb_values.
         * (* TWord *)
@@ -495,60 +477,10 @@ Section WithMap.
             rewrite word.unsigned_eqb;
             try rewrite word.unsigned_of_Z_0;
             now try rewrite word.unsigned_of_Z_1.
-    - (* ELet x e1 e2 *)
-      unfold compile_expr in He'.
-      fold (compile_expr (t := t1)) in He'.
-      fold (compile_expr (t := t2)) in He'.
-      fwd;
-      rename e into e1', e' into e2';
-      rename c0 into c1, c1 into c2;
-      rename r into nm1, r0 into nm2;
-      rename s into x', E1 into En;
-      rename E into E1, E0 into E2.
-      inversion He;
-      repeat lazymatch goal with
-      | h: existT _ _ _ = existT _ _ _ |- _ =>
-          apply Eqdep_dec.inj_pair2_eq_dec in h as [= ->]; try exact type_eq_dec
-      end;
-      subst;
-      rename H4 into He1, H6 into He2.
-      split.
-      { admit. }
+      + 
 
-      eapply exec.seq.
-      { apply IHe1 with (1 := Hlo) (2 := He1) (3 := E1) (4 := Hl). }
-      cbv beta.
-      intros tr' m' l' Hw.
-      fwd.
 
-      apply exec.seq with (mid := fun tr'' m'' l'' => m'' = m /\ l'' = map.put l' x' w).
-      {
-        eapply exec.set.
-        + exact Hwp0.
-        + now split.
-      }
-      intros tr'' m'' l'' Hw'.
-      fwd.
-      eassert (H : interp_expr lo (ELet x e1 e2) = interp_expr _ _) by now simpl.
-      rewrite H. clear H.
-
-      eapply exec.weaken.
-      {
-        apply IHe2 with (2 := He2) (3 := E2) (lo := (set_local lo x (interp_expr lo e1))).
-        + now apply tenv_relation_put.
-        + admit.
-      }
-      cbv beta.
-      intros tr''' m''' l''' [w0 H].
-      fwd.
-      exists w0. ssplit.
-      + easy.
-      + exact Hp1.
-      + reflexivity.
-      + apply extends_trans with (map.put l' x' w). { assumption. }
-        apply put_extends_l. 2: assumption.
-        admit.
-  Admitted.
+  Qed.
 
 End WithMap.
 
